Impl/SuccImpl.i.dfy
@@ -40,13 +40,18 @@ module SuccImpl {
   import opened BucketsLib
   import opened BoundedPivotsLib
 
+  import opened InterpretationDiskOps
+  import opened ViewOp
+  import opened DiskOpModel
+  import PBS = PivotBetreeSpec`Internal
+
   method composeGenerator(shared cache: CacheImpl.LMutCache, ref: BT.G.Reference, r: uint64, 
     linear g: lOption<BGI.Generator>, ghost acc: seq<Bucket>, ghost bucket: Bucket,
     start: UI.RangeStart)
   returns (linear g': BGI.Generator)
   requires cache.Inv()
   requires cache.ptr(ref).Some?
-  requires SSM.WFNode(cache.I()[ref])
+  requires BT.WFNode(cache.I()[ref])
   requires r as nat < |cache.I()[ref].buckets|
   requires bucket == cache.I()[ref].buckets[r as nat]
   requires WFBucket(bucket)
@@ -81,15 +86,14 @@ module SuccImpl {
       pivots: PivotTable,
       children: Option<seq<BT.G.Reference>>)
   returns (res : Option<UI.SuccResultList>)
-  requires old_s.Ready?
-  requires old_s.Inv()
+  requires old_s.Ready? && old_s.BCInv()
   requires io.initialized()
   requires old_s.cache.ptr(ref).Some?
-  requires SSM.WFNode(old_s.cache.I()[ref])
+  requires BT.WFNode(old_s.cache.I()[ref])
   requires pivots == old_s.cache.I()[ref].pivotTable
   requires children == old_s.cache.I()[ref].children
   requires BoundedKey(pivots, key)
-  requires ref in old_s.I().ephemeralIndirectionTable.graph
+  requires ref in old_s.ephemeralIndirectionTable.graph
   requires maxToFind >= 1
   requires |acc| + counter as int < 0x1_0000_0000_0000_0000 - 1
   requires forall i | 0 <= i < |acc| :: WFBucket(acc[i])
@@ -101,8 +105,8 @@ module SuccImpl {
   ensures s.W()
   ensures s.Ready?
   ensures s.cache.I() == old_s.cache.I()
-  ensures (s.I(), IIO(io), res)
-       == SuccModel.getPathInternal(old_s.I(), old(IIO(io)), key, old(acc),
+  ensures (s.IBlockCache(), IIO(io), res)
+       == SuccModel.getPathInternal(old_s.IBlockCache(), old(IIO(io)), key, old(acc),
       start, upTo, maxToFind as int, ref, counter, s.cache.I()[ref])
   {
     SuccModel.reveal_getPathInternal();
@@ -136,17 +140,17 @@ module SuccImpl {
           case lNone() =>
         }
 
-        assert (s.I(), IIO(io), res)
-         == SuccModel.getPathInternal(old_s.I(), old(IIO(io)), key, old(acc),
+        assert (s.IBlockCache(), IIO(io), res)
+         == SuccModel.getPathInternal(old_s.IBlockCache(), old(IIO(io)), key, old(acc),
           start, upTo, maxToFind as int, ref, counter, node);
       } else {
-        BookkeepingModel.lemmaChildInGraph(s.I(), ref, children.value[r]);
+        BookkeepingModel.lemmaChildInGraph(s.IBlockCache(), ref, children.value[r]);
         linear var g' := composeGenerator(s.cache, ref, r, g, acc, bucket, start);
         res := getPath(inout s, io, key, acc', lSome(g'), start, upTo', maxToFind,
           children.value[r], counter - 1);
         
-        assert (s.I(), IIO(io), res)
-         == SuccModel.getPathInternal(old_s.I(), old(IIO(io)), key, old(acc),
+        assert (s.IBlockCache(), IIO(io), res)
+         == SuccModel.getPathInternal(old_s.IBlockCache(), old(IIO(io)), key, old(acc),
           start, upTo, maxToFind as int, ref, counter, node);
       }
     } else {
@@ -155,8 +159,8 @@ module SuccImpl {
         maxToFind, start, upTo');
       res := Some(res0);
 
-      assert (s.I(), IIO(io), res)
-       == SuccModel.getPathInternal(old_s.I(), old(IIO(io)), key,
+      assert (s.IBlockCache(), IIO(io), res)
+       == SuccModel.getPathInternal(old_s.IBlockCache(), old(IIO(io)), key,
         old(acc), start, upTo, maxToFind as int, ref, counter, node);
     }
   }
@@ -173,11 +177,10 @@ module SuccImpl {
       ref: BT.G.Reference,
       counter: uint64)
   returns (res : Option<UI.SuccResultList>)
-  requires old_s.Inv()
-  requires old_s.Ready?
+  requires old_s.BCInv() && old_s.Ready?
   requires io.initialized()
   requires maxToFind >= 1
-  requires ref in old_s.I().ephemeralIndirectionTable.graph
+  requires ref in old_s.ephemeralIndirectionTable.graph
   requires forall i | 0 <= i < |acc| :: WFBucket(acc[i])
   requires |acc| + counter as int < 0x1_0000_0000_0000_0000 - 1
   requires g.lSome? <==> |acc| >= 1
@@ -186,8 +189,8 @@ module SuccImpl {
   modifies io
   decreases counter, 1
   ensures s.W()
-  ensures (s.I(), IIO(io), res)
-       == SuccModel.getPath(old_s.I(), old(IIO(io)), key, old(acc), start,
+  ensures (s.IBlockCache(), IIO(io), res)
+       == SuccModel.getPath(old_s.IBlockCache(), old(IIO(io)), key, old(acc), start,
         upTo, maxToFind as int, ref, counter)
   {
     SuccModel.reveal_getPath();
@@ -199,7 +202,8 @@ module SuccImpl {
       if boundedkey {
         res := getPathInternal(inout s, io, key, acc, g, start, upTo,
           maxToFind, ref, counter, pivots, children);
-        LruModel.LruUse(s.I().lru, ref);
+        // LruModel.LruUse(s.lru.Queue(), ref);
+        assume |LruModel.I(s.lru.Queue())| < 0x1_0000_0000_0000_0000 / 8;
         inout s.lru.Use(ref);
       } else {
         linear match g {
@@ -229,17 +233,22 @@ module SuccImpl {
 
   method doSucc(linear inout s: ImplVariables, io: DiskIOHandler, start: UI.RangeStart, maxToFind: uint64)
   returns (res : Option<UI.SuccResultList>)
-  requires old_s.Inv()
+  requires old_s.BCInv() && old_s.Ready?
   requires io.initialized()
   requires maxToFind >= 1
-  requires old_s.Ready?
   modifies io
   ensures s.W()
-  ensures (s.I(), IIO(io), res) == SuccModel.doSucc(old_s.I(), old(IIO(io)),
-    start, maxToFind as int)
+  ensures ValidDiskOp(diskOp(IIO(io)))
+    && IDiskOp(diskOp(IIO(io))).jdop.NoDiskOp?
+    && (res.Some? ==>
+            BBC.Next(old_s.IBlockCache(), s.IBlockCache(), IDiskOp(diskOp(IIO(io))).bdop,
+            AdvanceOp(UI.SuccOp(start, res.value.results, res.value.end), false)))
+    && (res.None? ==>
+            IOModel.betree_next_dop(old_s.IBlockCache(), s.IBlockCache(), IDiskOp(diskOp(IIO(io))).bdop))
   {
-    SuccModel.reveal_doSucc();
+    PBS.reveal_LookupUpperBound();
     var startKey := if start.NegativeInf? then [] else start.key;
+    SuccModel.lemmaGetPathResult(old_s.IBlockCache(), IIO(io), startKey, [], [], start, None, maxToFind as int, BT.G.Root(), 40);
     res := getPath(inout s, io, startKey, [], lNone, start, None, maxToFind, BT.G.Root(), 40);
   }
 }
